@prefix dc:    <http://purl.org/dc/terms/> .
@prefix rdfs:  <http://www.w3.org/2000/01/rdf-schema#> .
@prefix foaf:  <http://xmlns.com/foaf/0.1/> .
@prefix owl:   <http://www.w3.org/2002/07/owl#> .
@prefix sd:    <http://www.w3.org/ns/sparql-service-description#> .
@prefix rdf:   <http://www.w3.org/1999/02/22-rdf-syntax-ns#> .

<http://lsq.aksw.org/vocab#meanTriplePatternSelectivity>
        a             owl:DatatypeProperty ;
        rdfs:comment  "The mean selectivity of all triple patterns"@en ;
        rdfs:label    "mean selectivity of triple patterns"@en ;
        rdfs:range    <http://www.w3.org/2001/XMLSchema#decimal> .

<http://lsq.aksw.org/vocab#mentionsSubject>
        a             rdf:Property ;
        rdfs:comment  "Links a query to a term it mentions in the subject of a triple pattern"@en ;
        rdfs:label    "mentions subject"@en .

<http://lsq.aksw.org/vocab#executionError>
        a             owl:DatatypeProperty ;
        rdfs:comment  "The text of an error encountered during a query execution"@en ;
        rdfs:label    "execution error"@en .

<http://lsq.aksw.org/vocab#mentionsPredicate>
        a             rdf:Property ;
        rdfs:comment  "Links a query to a term it mentions in the predicate of a triple pattern"@en ;
        rdfs:label    "mentions predicate"@en .

<http://lsq.aksw.org/vocab#Regex>
        a           sd:Feature ;
        rdfs:label  "Regex"@en .

<http://lsq.aksw.org/vocab#Execution>
        a             owl:Class ;
        rdfs:comment  "Each instance is an execution of a particular query against a particular endpoint at a particular time by a particular agent"@en ;
        rdfs:label    "Query Execution"@en .

<http://lsq.aksw.org/vocab#Sink>
        a                owl:Class ;
        rdfs:comment     "Each instance is a sink join vertex (position) in the query (multiple incoming edges, zero outgoing edges)"@en ;
        rdfs:label       "Sink Join Vertex"@en ;
        rdfs:subClassOf  <http://lsq.aksw.org/vocab#JoinVertex> .

<http://lsq.aksw.org/vocab#Minus>
        a           sd:Feature ;
        rdfs:label  "Minus"@en .

<http://lsq.aksw.org/vocab#Count>
        a           sd:Feature ;
        rdfs:label  "Count"@en .

<http://lsq.aksw.org/vocab#Values>
        a           sd:Feature ;
        rdfs:label  "Values"@en .

<http://lsq.aksw.org/vocab#usesFeature>
        a             owl:ObjectProperty ;
        rdfs:comment  "A feature used by the query"@en ;
        rdfs:label    "uses feature"@en .

<http://lsq.aksw.org/vocab#joinVertex>
        a             owl:ObjectProperty ;
        rdfs:comment  "Links a query to a join vertex it contains"@en ;
        rdfs:label    "has join vertex"@en .

<http://lsq.aksw.org/vocab#Offset>
        a           sd:Feature ;
        rdfs:label  "Offset"@en .

<http://lsq.aksw.org/vocab#parseError>
        a             owl:DatatypeProperty ;
        rdfs:comment  "The text of an error encountered when parsing query"@en ;
        rdfs:label    "parse error"@en .

<http://lsq.aksw.org/vocab#triplePatterns>
        a             owl:FunctionalProperty , owl:DatatypeProperty ;
        rdfs:comment  "The number of triple patterns in a query"@en ;
        rdfs:label    "number of triple patterns"@en ;
        rdfs:range    <http://www.w3.org/2001/XMLSchema#nonNegativeInteger> .

<http://lsq.aksw.org/vocab#resultSize>
        a             owl:DatatypeProperty ;
        rdfs:comment  "Number of results returned when executed locally"@en ;
        rdfs:label    "result size"@en ;
        rdfs:range    <http://www.w3.org/2001/XMLSchema#nonNegativeInteger> .

<http://lsq.aksw.org/vocab#Filter>
        a           sd:Feature ;
        rdfs:label  "Filter"@en .

<http://lsq.aksw.org/vocab#Hybrid>
        a                owl:Class ;
        rdfs:comment     "Each instance is a hybrid join vertex (position) in the query (at least one incoming edge, at least one outgoing edge, at least three edges)"@en ;
        rdfs:label       "Hybrid Join Vertex"@en ;
        rdfs:subClassOf  <http://lsq.aksw.org/vocab#JoinVertex> .

<http://lsq.aksw.org/vocab#runTimeMs>
        a             owl:DatatypeProperty ;
        rdfs:comment  "The run time of the query in milliseconds when executed locally"@en ;
        rdfs:label    "run time in milliseconds"@en ;
        rdfs:range    <http://www.w3.org/2001/XMLSchema#decimal> .

<http://lsq.aksw.org/vocab#Distinct>
        a           sd:Feature ;
        rdfs:label  "Distinct"@en .

<http://lsq.aksw.org/vocab#SubQuery>
        a           sd:Feature ;
        rdfs:label  "SubQuery"@en .

<http://lsq.aksw.org/vocab#Limit>
        a           sd:Feature ;
        rdfs:label  "Limit"@en .

<http://lsq.aksw.org/vocab#Star>
        a                owl:Class ;
        rdfs:comment     "Each instance is a star-shaped join vertex (position) in the query (zero incoming edges, multiple outgoing edges)"@en ;
        rdfs:label       "Star Join Vertex"@en ;
        rdfs:subClassOf  <http://lsq.aksw.org/vocab#JoinVertex> .

<http://lsq.aksw.org/vocab#Optional>
        a           sd:Feature ;
        rdfs:label  "Optional"@en .

<http://lsq.aksw.org/vocab#Sum>
        a           sd:Feature ;
        rdfs:label  "Sum"@en .

<http://lsq.aksw.org/vocab#execution>
        a             owl:FunctionalProperty , owl:ObjectProperty ;
        rdfs:comment  "Links a query to an execution of it against a particular endpoint by a particular agent at a particular time"@en ;
        rdfs:label    "has execution"@en .

<http://lsq.aksw.org/vocab#meanJoinVerticesDegree>
        a             owl:FunctionalProperty , owl:DatatypeProperty ;
        rdfs:comment  "The mean degree across all the join vertices"@en ;
        rdfs:label    "mean join vertex degree"@en ;
        rdfs:range    <http://www.w3.org/2001/XMLSchema#decimal> .

<http://lsq.aksw.org/vocab#bgps>
        a             owl:FunctionalProperty , owl:DatatypeProperty ;
        rdfs:comment  "The number of Basic Graph Patterns in a query"@en ;
        rdfs:label    "number of bgps"@en ;
        rdfs:range    <http://www.w3.org/2001/XMLSchema#nonNegativeInteger> .

<http://lsq.aksw.org/vocab#spinError>
        a             owl:DatatypeProperty ;
        rdfs:comment  "The text of an error encountered when generating the SPIN description"@en ;
        rdfs:label    "SPIN error"@en .

<http://lsq.aksw.org/vocab#Union>
        a           sd:Feature ;
        rdfs:label  "Union"@en .

<http://lsq.aksw.org/vocab#FromNamed>
        a           sd:Feature ;
        rdfs:label  "FromNamed"@en .

<http://lsq.aksw.org/vocab#joinVertexType>
        a             owl:FunctionalProperty , owl:ObjectProperty ;
        rdfs:comment  "Links a join vertex to the type of vertex it is"@en ;
        rdfs:label    "is of type"@en .

<http://lsq.aksw.org/vocab#joinVertices>
        a             owl:FunctionalProperty , owl:DatatypeProperty ;
        rdfs:comment  "The number of join vertices in a query"@en ;
        rdfs:label    "number of join vertices"@en ;
        rdfs:range    <http://www.w3.org/2001/XMLSchema#nonNegativeInteger> .

<http://lsq.aksw.org/vocab#JoinVertex>
        a             owl:Class ;
        rdfs:comment  "Each instance is a join vertex (position) in the query"@en ;
        rdfs:label    "Join Vertex"@en .

<http://lsq.aksw.org/vocab#Path>
        a                owl:Class ;
        rdfs:comment     "Each instance is a path-shaped join vertex (position) in the query (one incoming edge, one outgoing edge)"@en ;
        rdfs:label       "Path Join Vertex"@en ;
        rdfs:subClassOf  <http://lsq.aksw.org/vocab#JoinVertex> .

<http://lsq.aksw.org/vocab#GroupBy>
        a           sd:Feature ;
        rdfs:label  "GroupBy"@en .

<http://lsq.aksw.org/vocab#Avg>
        a           sd:Feature ;
        rdfs:label  "Avg"@en .

<http://lsq.aksw.org/vocab#endpoint>
        a             owl:FunctionalProperty , owl:ObjectProperty ;
        rdfs:comment  "Links a query execution instance to the endpoint against which it was run"@en ;
        rdfs:label    "run at endpoint"@en .

<http://lsq.aksw.org/vocab#runtimeError>
        a             owl:DatatypeProperty ;
        rdfs:comment  "The text of an error encountered when running the query locally"@en ;
        rdfs:label    "runtime error"@en .

<http://lsq.aksw.org/vocab#Having>
        a           sd:Feature ;
        rdfs:label  "Having"@en .

<http://lsq.aksw.org/vocab#mentionsObject>
        a             rdf:Property ;
        rdfs:comment  "Links a query to a term it mentions in the object of a triple pattern"@en ;
        rdfs:label    "mentions object"@en .

<http://lsq.aksw.org/vocab#Max>
        a           sd:Feature ;
        rdfs:label  "Max"@en .

<http://lsq.aksw.org/vocab#NamedGraph>
        a           sd:Feature ;
        rdfs:label  "NamedGraph"@en ;
        owl:sameAs  <http://lsq.aksw.org/vocab#namedGraph> .

<http://lsq.aksw.org/vocab#agent>
        a             owl:FunctionalProperty , owl:ObjectProperty ;
        rdfs:comment  "Links a query execution instance to the agent that initiated the execution"@en ;
        rdfs:label    "run by agent"@en .

<http://lsq.aksw.org/vocab#Service>
        a           sd:Feature ;
        rdfs:label  "Service"@en .

<http://lsq.aksw.org/vocab#Min>
        a           sd:Feature ;
        rdfs:label  "Min"@en .

<http://lsq.aksw.org/vocab#OrderBy>
        a           sd:Feature ;
        rdfs:label  "OrderBy"@en .

<http://lsq.aksw.org/vocab>
        a               owl:Ontology ;
        dc:creator      <http://aidanhogan.com/foaf.rdf#me> ;
        dc:date         "2015-09-07Z"^^<http://www.w3.org/2001/XMLSchema#date> ;
        dc:description  "The Linked SPARQL Queries Vocabulary (LSQ(V)), defined using RDF(S) and OWL, provides a machine readable vocabulary to help describe queries in SPARQL logs and their statistics. The vocabulary builds upon the SPIN vocabulary and the Service Description vocabulary."@en ;
        dc:title        "The Linked SPARQL Queries Vocabulary (LSQ(V))"@en .

<http://lsq.aksw.org/vocab#Bind>
        a           sd:Feature ;
        rdfs:label  "Bind"@en .
